greve day commit [1]

code/experimental/P256/Hacl.Impl.LowLevel.fst
@@ -538,15 +538,23 @@ let mod64 a = index a (size 0)
 
 
 val shortened_mul: a: ilbuffer uint64 (size 4) -> b: uint64 -> result: widefelem -> Stack unit
-  (requires fun h -> live h a /\ live h result)
+  (requires fun h -> live h a /\ live h result /\ wide_as_nat h result = 0)
   (ensures fun h0 _ h1 -> modifies (loc result) h0 h1 /\ 
-    felem_seq_as_nat (as_seq h0 a) * uint_v b = wide_as_nat h1 result /\ wide_as_nat h1 result < pow2 320)
+    as_nat_il h0 a * uint_v b = wide_as_nat h1 result /\ 
+    wide_as_nat h1 result < pow2 320)
 
 let shortened_mul a b result = 
-    let result04 = sub result (size 0) (size 4) in 
-    let c = mul1_il a b result04 in 
-    admit();
-  upd result (size 4) c
+  let result04 = sub result (size 0) (size 4) in 
+  let result48 = sub result (size 4) (size 4) in 
+  let c = mul1_il a b result04 in 
+    let h0 = ST.get() in 
+  upd result (size 4) c;
+  
+    assert(Lib.Sequence.index (as_seq h0 result) 5 == Lib.Sequence.index (as_seq h0 result48) 1);
+    assert(Lib.Sequence.index (as_seq h0 result) 6 == Lib.Sequence.index (as_seq h0 result48) 2);
+    assert(Lib.Sequence.index (as_seq h0 result) 7 == Lib.Sequence.index (as_seq h0 result48) 3);
+
+    assert_norm( pow2 64 * pow2 64 * pow2 64 * pow2 64 = pow2 256)
    
 
 val shift8: t: widefelem -> t1: widefelem -> Stack unit 
